update

cava2/Components/RealignMaskedFifoProperties.v
@@ -56,13 +56,6 @@ Section RealignMaskedFifo.
   Existing Instance fifo_correctness.
   Existing Instance realign_specification.
   Existing Instance realign_correctness.
-  Set Typeclasses Debug.
-
-
-  Lemma concat_bytes_resize xs:
-    length xs <= 4 -> BigEndianBytes.concat_bytes (List.resize Byte.x00 4 xs)
-                 = BigEndianBytes.concat_bytes xs.
-  Admitted.
 
   Global Instance realign_masked_fifo_invariant
   : invariant_for (realign_masked_fifo fifo_size) (list N * (bool * list Byte.byte * list Byte.byte)) :=
@@ -117,8 +110,41 @@ Section RealignMaskedFifo.
       ;
 
      postcondition :=
-      fun input contents (output: denote_type (output_of (realign_masked_fifo fifo_size))) =>
-        True;
+      fun input '(fifo_contents, realign_contents) (output: denote_type (output_of (realign_masked_fifo fifo_size))) =>
+      let '(data_valid, (data, (data_mask, (drain, (consumer_ready, tt))))) := input in
+
+      let fifo_empty := (length fifo_contents =? 0) in
+      let fifo_full := (length fifo_contents =? fifo_size) in
+
+      let realign_input :=
+        (data_valid, (data, (data_mask, (drain && fifo_empty && consumer_ready, (negb fifo_full, tt))))) in
+      let '(realign_valid, (realign_data, realign_len)) :=
+        realign_spec (fst (fst realign_contents)) (snd (fst realign_contents)) (snd realign_contents) realign_input in
+
+      let fifo_input :=
+        (realign_valid && negb drain && negb fifo_full, (realign_data, (consumer_ready, tt))) in
+
+      let new_fifo_contents :=
+        update_repr (c:=fifo (T:=BitVec 32) fifo_size) fifo_input fifo_contents in
+
+      let fifo_full := (length new_fifo_contents =? fifo_size) in
+      let fifo_valid := 1 <=? length fifo_contents in
+
+      let valid :=
+        if drain then fifo_valid || realign_valid else fifo_valid in
+
+      let data :=
+        if drain && negb fifo_valid then realign_data
+        else hd default fifo_contents in
+      let length :=
+        if drain && negb fifo_valid then realign_len
+        else 4%N in
+
+      if valid then
+        output = (valid, (data, (length, (drain && negb fifo_valid && valid, fifo_full))))
+      else
+        exists unknown,
+        output = (valid, (unknown, (length, (drain && negb fifo_valid && valid, fifo_full))));
   |}%nat.
 
   Lemma realign_masked_fifo_invariant_preserved : invariant_preserved (realign_masked_fifo fifo_size).
@@ -162,18 +188,16 @@ Section RealignMaskedFifo.
       simplify_spec (fifo (T:=BitVec 32) fifo_size).
       cbv [realign_update_latched_valid realign_update_latched_bytes realign_spec] in *.
       autorewrite with tuple_if; cbn [fst snd]; destruct fifo_full; boolsimpl.
-      { destruct (length new_fifo_contents =? fifo_size); boolsimpl; try reflexivity.
+      { destr (length new_fifo_contents =? fifo_size); boolsimpl; try reflexivity.
         {
           revert H4; rewrite H2.
           destr (fifo_size =? 0); boolsimpl; try lia.
-          destruct ((4 <=? length new_realign_ghost) && negb drain).
-          { intros. lia. }
-          { reflexivity. }
         }
       }
-      { destruct (length new_fifo_contents =? fifo_size); boolsimpl; try reflexivity.
-        destruct fifo_empty; destruct (length new_fifo_contents =? 0); boolsimpl; try reflexivity;
-          destruct drain; boolsimpl; try reflexivity;
+      { cbn [denote_type].
+        destr (length new_fifo_contents =? fifo_size); boolsimpl; try reflexivity.
+        destr fifo_empty; destr (length new_fifo_contents =? 0); boolsimpl; try reflexivity;
+          destruct drain; boolsimpl; try reflexivity; try lia;
           (destr (4 <=? length new_realign_ghost); [|reflexivity]); now rewrite resize_firstn_alt by lia.
       }
     }
@@ -182,7 +206,7 @@ Section RealignMaskedFifo.
       simplify_spec (realign_masked_fifo fifo_size).
       simplify_spec realign.
       simplify_invariant realign.
-      cbn [fst snd].
+      cbn [fst snd denote_type] in *.
       cbv [realign_update_latched_valid realign_update_latched_bytes realign_update_state].
       autorewrite with tuple_if; cbn [fst snd];
         destruct fifo_full; try rewrite H2; try rewrite Nat.eqb_refl;
@@ -192,674 +216,167 @@ Section RealignMaskedFifo.
       destr (length new_fifo_contents =? 0); try lia; boolsimpl.
       reflexivity.
     }
-    { admit. }
-    {
-      simplify_spec (realign_masked_fifo fifo_size).
-      simplify_spec realign.
-      assert ( (length new_fifo_contents =? fifo_size) = fifo_full).
-      { destruct fifo_full; subst.
-        { now rewrite Nat.eqb_refl. }
-        { apply Nat.eqb_neq. lia. }
-      }
-      assert ( (length new_fifo_contents =? 0) = fifo_empty).
-      { destruct fifo_empty.
-        { rewrite H3. now rewrite Nat.eqb_refl. }
-        { apply Nat.eqb_neq. lia. }
-      }
-      rewrite H6, H7 in H4.
-      cbn [realign_spec].
-      use_correctness' realign.
-      rewrite H5.
-      boolsimpl.
-      destruct fifo_full; destruct fifo_empty.
-      try rewrite H2, H3, Nat.eqb_refl in *.
-      {
-      rewrite H5.
-      autorewrite with tuple_if.
-      (* autorewrite with tuple_if; cbn [fst snd]; *)
-      cbv
-      destruct fifo_full; try rewrite H2; try rewrite Nat.eqb_refl;
-        boolsimpl; push_length.
-      rewrite
-      use_correctness' (fifo (T:= BitVec 32) fifo_size).
-      cbn [fst snd].
-
-  Admitted.
-
-
-
-
-    logical_simplify.
-    stepsimpl.
-    repeat (destruct_pair_let ; cbn [fst snd]).
-    cbn [denote_type absorb_any] in *.
-    ssplit.
-    {
-      apply step_fifo_invariant with (contents:=fifo_contents).
-      { apply Hfifo_nz. }
-      { now apply Hnew_fifo_contents. }
-      { cbv [fifo_pre].
-        destruct fifo_state as (?,(?,(?,count))).
-        destruct fifo_full.
-        { now boolsimpl. }
-        { boolsimpl.
-          cbv [fifo_invariant] in H.
-          logical_simplify.
-          rewrite H4.
-          match goal with
-          | |- if ?B then _ else _ => destruct B
-          end.
-          { apply H1. }
-          trivial.
-          }
-      }
-      apply H.
-    }
-
-      {
-        destruct r.
-        eapply (invariant_preserved_pf (c:=fifo fifo_size) ).
-        2:{
-          cbn [denote_type] in *; destruct_products.
-          cbn [fst snd].
-          apply H0l. }
-        2:{
-          cbv [precondition fifo_specification].
-          (* cbn [absorb_any] in *. *)
-          pose tktktk as H.
-          (* pose proof (output_correct_pf (c:=realign)). *)
-          cbv [output_correct postcondition realign_specification] in H.
-          cbn [denote_type absorb_any] in *.
-          (* destruct input as (?, (?, (?, (?, (?, ?))))). *)
-          destruct input as (data_valid, (data, (data_mask, (drain, (consumer_ready, []))))).
-          cbn [fst snd].
-          specialize (H
-            (data_valid,
-            (data,
-            (data_mask,
-            (drain && fst (snd (snd (snd (snd (fst state))))) && consumer_ready,
-            (negb (snd (snd (snd (snd (snd (fst state)))))), tt)))))).
-          specialize (H (fst (snd state))).
-          destruct H.
-          (* assert (bool * list Byte.byte * list Byte.byte) by admit. *)
-
-          (* specialize (H H2). *)
-          assert (realign_invariant (fst (snd state)) x) .
-          { cbv [realign_invariant]. destruct x as ((?,?),?).
-            cbv [realign_invariant'].
-            destruct state as (state, (realign_state, fifo_state)).
-            destruct realign_state as (out_valid, (out_data, (out_len, (buff, buff_len)))).
-            cbn [fst snd].
-
-          specialize (H H3).
-          assert (
-           precondition realign
-  (data_valid,
-           (data,
-           (data_mask,
-           (drain && fst (snd (snd (snd (snd (fst state))))) && consumer_ready,
-           (negb (snd (snd (snd (snd (snd (fst state)))))), tt)))))
-             H2) by admit.
-          specialize (H H4).
-          destruct H2 as ((latched_valid, latched_bytes), ghost_state).
-          cbn [absorb_any denote_type] in *.
-          rewrite H.
-          cbv [realign_spec].
-          destruct state as (state, (realign_state, fifo_state)).
-          destruct state as (is_last, (out_valid, (out_data, (out_length, (fifo_empty, fifo_full))))).
-          (* destruct_products. *)
-          autorewrite with tuple_if.
-          cbn [fst snd negb];
-          cbv [fifo_invariant] in H0.
-          destruct fifo_state as (?, (?, (fifo, count))).
-          logical_simplify.
-          destruct fifo_full; boolsimpl.
-          { trivial. }
-          destruct (
-           ((4 <=? length ghost_state)
-            || drain && fifo_empty && consumer_ready && (1 <=? length ghost_state)) && negb drain).
-          { apply H5. }
-          trivial.
-        }
-        cbv [update_repr realign_masked_fifo_specification fifo_specification].
-        destruct input as (data_valid, (data, (data_mask, (drain, (consumer_ready, []))))).
-        destruct state as (state, (realign_state, fifo_state)).
-        destruct state as (is_last, (out_valid, (out_data, (out_length, (fifo_empty, fifo_full))))).
-        cbn [fst snd].
-
-
-
-
-        realign_invariant (fst (snd state)) H2) by admit.
-
-
-        destruct_products.
-        rewrite H2.
-
-        match goal with
-        | |- context [step ?c ?s ?i]=>
-          (* idtac *)
-          (* assert ( realign_invariant d10 p) by admit; *)
-          (* assert ( realign_pre (d, (d0, (d1, (d2 && d8 && fst d3, (negb d9, tt))))) ) by admit; *)
-          (* pose proof (output_correct_pf (c:=c) i s p (ltac:(eauto)) (ltac:(eauto))) *)
-          (* generalize dependent (snd (step c s i)); intros; *)
-          (* simplify_spec c; logical_simplify *)
-        end.
-        destruct p as ((?,?),?).
-        destruct p.
-
-        subst.
-
-
-
-    rewrite (surjective_pairing (step c s i));
-          use_correctness.
-
-        }
-        admit. }
-      {
-        rewrite (surjective_pairing (step c s i));
-
-        use_correctness' realign.
-
-        cbv [ update_repr realign_masked_fifo_specification fifo_specification].
-
-        match goal with
-        | |- context [ step realign ?X ?Y ] =>
-          remember (step realign X Y);
-          pose proof (output_correct_pf (c:=realign) Y X (false, [], l0))
-        end.
-        destruct p as ((?,?),?).
-        intros.
-        cbn [absorb_any] in *.
-        specialize (H X).
-
-        (* simplify_spec (fifo (T:=BitVec 32) fifo_size). *)
-        simplify_spec realign.
-
-        destruct enable; [ | reflexivity ].
-        change (2 ^ 8) with 256 in *. change (2 ^ 16) with 65536 in *.
-        Zify.zify. Z.to_euclidean_division_equations. lia. }
-        repeat (destruct_pair_let; cbn [fst snd]).
-        destruct realign_masked_fifo_specification.
-        destruct fifo_specification.
-        cbv [ update_repr].
-
-      cbv [invariant_preserved]. intros (enable,[]) (data,?) value.
-      intros; subst. simplify_invariant double_counter.
-      cbv [double_counter]. stepsimpl. logical_simplify; subst.
-      repeat use_correctness. stepsimpl.
-      simplify_spec double_counter.
-      ssplit.
-      { eapply (invariant_preserved_pf (c:=counter));
-          [ | solve [eauto] .. ].
-        simplify_spec counter.
-        destruct enable; [ | reflexivity ].
-        change (2 ^ 8) with 256 in *. change (2 ^ 16) with 65536 in *.
-
-
-      use_correctness' (fifo (T:=BitVec 32) fifo_size). stepsimpl.
-      simplify_spec (realign_masked_fifo fifo_size).
-      ssplit.
-
-      (* simplify_invariant double_counter. *)
-      (* simplify_spec double_counter. *)
-      (* intros; logical_simplify; subst. *)
-      (* cbv [double_counter]. stepsimpl. *)
-      (* repeat use_correctness. stepsimpl. *)
-      (* f_equal. *)
-
-
-    (* cbv [fifo_invariant]. cbn [absorb_any]. *)
-    simplify_spec (realign_masked_fifo fifo_size).
-    intros.
-    destruct r.
-    destruct new_r.
-    destruct input as (data_valid, (data, (data_mask, (drain, (consumer_ready, []))))).
-    destruct state as (state, (realign_state, fifo_state)).
-    inversion H; clear H.
-    destruct state as (is_last, (out_valid, (out_data, (out_length, (fifo_empty, fifo_full))))).
-    destruct fifo_state as (?, (?, (?, ?))).
-    subst; intros.
-    logical_simplify.
-    intros.
-    repeat (destruct_pair_let; cbn [fst snd]).
-    cbv [realign_masked_fifo]; stepsimpl.
-    repeat (destruct_pair_let; cbn [fst snd]).
-    (* Check fifo. *)
-    eapply (invariant_preserved_pf (c:=fifo fifo_size)).
-    {
-      cbv [update_repr].
-      cbv [fifo_specification].
-      cbv [fifo_invariant] in H0.
-      (* Set Printing Implicit. *)
-      (* match goal with *)
-      (* | |- context [?X] => *)
-      (*   match X with *)
-      (*   | snd (step realign _ _) => remember X as p *)
-      (*   end *)
-      (* end. *)
-
-      (* revert Heqp. *)
-    (* simplify_spec realign. *)
-
-    (* Existing Instance realign_. *)
-
-    lazymatch goal with
-    | |- context [snd (step realign ?s ?i)] =>
-      find_correctness realign;
-      pose proof (output_correct_pf (c:=realign) i s)
-    end.
-
-    specialize (H (true, [], l0)).
-
-    use_correctness' realign.
-    pose proof (output_correct_pf (c:=realign) _ _ ).
-    generalize dependent (snd (step realign realign_state
-     (data_valid,
-     (data,
-     (data_mask,
-     (drain && fifo_empty && consumer_ready, (negb fifo_full, tt))))))
-    ); intros.
-    revert H.
-    simplify_invariant realign; intros. specialize (H X).  subst. logical_simplify; subst
-    use_correctness' realign.
-
-    stepsimpl.
-
-      cbn [update_repr].
-    eappy
-    kcbn [fst snd].
-    logical_simplify.
-    repeat use_correctness. stepsimpl.
-    ssplit.
-
-
-
-      (* cbv [invariant_preserved]. intros (enable,[]) (data,?) value. *)
-      (* intros; subst. simplify_invariant double_counter. *)
-      (* cbv [double_counter]. stepsimpl. logical_simplify; subst. *)
-      repeat use_correctness. stepsimpl.
-      simplify_spec double_counter.
-      ssplit.
-          [ | solve [eauto] .. ].
-        simplify_spec counter.
-        destruct enable; [ | reflexivity ].
-
-
-
-    cbv [realign_masked_fifo K]. stepsimpl. ; subst; intros.
-    cbv [Fifo.fifo K]; stepsimpl; push_length.
-    autorewrite with Nnat.
-    subst.
-    cbv []
-    intros; logical_simplify; revert H0; subst; intros.
-
-  (* Specification for the 'realign_masked_fifo' component defined in terms of
-   * 'fifo_spec' and 'realign_masked_spec'. *)
-  Definition realign_masked_fifo_spec
-    fifo_contents
-    realign_masked_state
-    (input : denote_type (input_of (var:=denote_type) (realign_masked_fifo fifo_size))) :=
-    let '(data_valid, (data, (data_mask, (drain, (consumer_ready, tt))))) := input in
-
-    let fifo_empty := (length fifo_contents =? 0) in
-    let fifo_full := (length fifo_contents =? fifo_size) in
-
-    let realign_masked_input := (data_valid, (data, (data_mask, ((drain && fifo_empty && consumer_ready), (negb fifo_full, tt))))) in
-
-    let '(realign_maskeded_valid, (realign_maskeded_data, realign_maskeded_length)) :=
-      realign_spec
-        (fst (fst realign_masked_state)) (snd (fst realign_masked_state)) (snd realign_masked_state)
-        realign_masked_input
-    in
-
-    let fifo_input := ( (realign_maskeded_valid && (negb drain) && (negb fifo_full)), (realign_maskeded_data, (consumer_ready, tt))) in
-
-    let new_contents :=
-      fifo_contents_update (BitVec 32) fifo_size
-        fifo_empty fifo_full fifo_contents fifo_input
-    in
-
-    let '(fifo_valid, (fifo_data, (fifo_empty, fifo_full))) :=
-      fifo_spec (BitVec 32) fifo_size
-        fifo_contents new_contents fifo_input in
-
-    let valid :=
-      if drain then fifo_valid || realign_maskeded_valid else fifo_valid in
-    let data :=
-      if drain && negb fifo_valid then realign_maskeded_data
-      else fifo_data in
-    let length :=
-      if drain && negb fifo_valid then realign_maskeded_length
-      else 4%N in
-
-    (valid, (data, (length, (drain && negb fifo_valid && valid, fifo_full)))).
-
-  (* Invariant for the 'realign_masked_fifo' component. *)
-  Definition realign_masked_fifo_invariant
-    fifo_contents realign_masked_contents
-    (state : denote_type (state_of (var:=denote_type) (realign_masked_fifo fifo_size))) :=
-
-    let '(top_state, (realign_masked_state, fifo_state)) := state in
-    let '(is_last, (out_valid, (out_data, (out_length, (fifo_empty, fifo_full))))) := top_state in
-
-    fifo_invariant (BitVec 32) fifo_size fifo_contents fifo_state
-    /\ realign_masked_invariant (fst (fst realign_masked_contents)) (snd (fst realign_masked_contents)) (snd realign_masked_contents) realign_masked_state
-    (* the only additional invariant we preserve is that we respect fifo_full &
-     * fifo_empty *)
-    /\ (if fifo_full then fifo_size = length fifo_contents else length fifo_contents < fifo_size)
-    /\ (if fifo_empty then length fifo_contents = 0 else length fifo_contents <> 0).
-
-
-  (* Precondition for the 'realign_masked_fifo' component. *)
-  Definition realign_masked_fifo_pre
-    (input : denote_type (input_of (realign_masked_fifo fifo_size)))
-    (state: denote_type (state_of (realign_masked_fifo fifo_size)))
-    :=
-    let '(valid, (data, _)) := input in
-    let '(_, (realign_masked_state, fifo_state)) := state in
-    let '(_, (_, (_, count))) := fifo_state in
-    (if valid then N.to_nat count < fifo_size else True)
-    /\ (data < 2 ^ 32)%N.
-
-  (* "fifo" state update, not intended to be readable,
-     discovered mechanically during the proof below. *)
-  Definition realign_masked_fifo_update_fifo_contents
-    fifo_contents
-    (input : denote_type (input_of (realign_masked_fifo fifo_size)))
-    (state : denote_type (state_of (realign_masked_fifo fifo_size))):=
-    fifo_contents_update (BitVec 32) fifo_size (length fifo_contents =? 0)
-      (length fifo_contents =? fifo_size) fifo_contents
-      (fst
-         (snd
-            (step realign_masked (fst (snd state))
-               (fst input,
-               (fst (snd input),
-               (fst (snd (snd input)),
-               (fst (snd (snd (snd input))) &&
-                fst (snd (snd (snd (snd (fst state))))) &&
-                fst (snd (snd (snd (snd input)))),
-               (negb (snd (snd (snd (snd (snd (fst state)))))), tt))))))) &&
-       negb (fst (snd (snd (snd input)))) &&
-       negb (snd (snd (snd (snd (snd (fst state)))))),
-      (fst
-         (snd
-            (snd
-               (step realign_masked (fst (snd state))
-                  (fst input,
-                  (fst (snd input),
-                  (fst (snd (snd input)),
-                  (fst (snd (snd (snd input))) &&
-                   fst (snd (snd (snd (snd (fst state))))) &&
-                   fst (snd (snd (snd (snd input)))),
-                  (negb (snd (snd (snd (snd (snd (fst state)))))), tt)))))))),
-      (fst (snd (snd (snd (snd input)))), tt))).
-
-  (* "realign_masked" state update, not intended to be readable,
-     discovered mechanically during the proof below. *)
-  Definition realign_masked_fifo_update_realign_masked_contents
-    realign_masked_contents
-    (input : denote_type (input_of (realign_masked_fifo fifo_size)))
-    (state : denote_type (state_of (realign_masked_fifo fifo_size))) :=
-    let '(top_state, _) := state in
-    let '(is_last, (out_valid, (out_data, (out_length, (fifo_empty, fifo_full))))) := top_state in
-    ( (
-      realign_masked_update_latched_valid (fst (fst realign_masked_contents)) (snd realign_masked_contents)
-        (fst input,
-        (fst (snd input),
-        (fst (snd (snd input)),
-        (fst (snd (snd (snd input))) && fifo_empty &&
-         fst (snd (snd (snd (snd input)))), (negb fifo_full, tt))))),
-      realign_masked_update_latched_bytes (snd (fst realign_masked_contents)) (snd realign_masked_contents)
-        (fst input,
-        (fst (snd input),
-        (fst (snd (snd input)),
-        (fst (snd (snd (snd input))) && fifo_empty &&
-         fst (snd (snd (snd (snd input)))), (negb fifo_full, tt)))))
-      ),
-      realign_masked_update_state (snd realign_masked_contents)
-        (fst input,
-        (fst (snd input),
-        (fst (snd (snd input)),
-        (fst (snd (snd (snd input))) && fifo_empty &&
-         fst (snd (snd (snd (snd input)))), (negb fifo_full, tt)))))
-    ).
-
-
-  Lemma step_realign_masked_fifo_invariant
-      fifo_contents
-      realign_masked_contents
-      new_fifo_contents
-      new_realign_masked_contents
-      (input : denote_type (input_of (realign_masked_fifo fifo_size)))
-      (state : denote_type (state_of (realign_masked_fifo fifo_size))):
-
-    new_fifo_contents = realign_masked_fifo_update_fifo_contents fifo_contents input state ->
-    new_realign_masked_contents = realign_masked_fifo_update_realign_masked_contents realign_masked_contents input state ->
-
-    realign_masked_fifo_pre input state ->
-    realign_masked_fifo_invariant fifo_contents realign_masked_contents state ->
-    realign_masked_fifo_invariant new_fifo_contents new_realign_masked_contents (fst (step (realign_masked_fifo fifo_size) state input)).
-  Proof.
-    cbv [realign_masked_fifo_invariant realign_masked_fifo].
-    destruct state as (top_state, (realign_masked_state, fifo_state)).
-    destruct realign_masked_state as (x0,(x1,(x2,(x3,x4)))).
-    destruct top_state as (is_last, (out_valid, (out_data, (out_length, (fifo_empty, fifo_full))))).
-
-    intros Hnew_fifo_contents Hnew_realign_masked_contents Hpre H.
-    logical_simplify.
-    stepsimpl.
-    repeat (destruct_pair_let ; cbn [fst snd]).
-    cbn [denote_type absorb_any] in *.
-    ssplit.
-    {
-      apply step_fifo_invariant with (contents:=fifo_contents).
-      { apply Hfifo_nz. }
-      { now apply Hnew_fifo_contents. }
-      { cbv [fifo_pre].
-        destruct fifo_state as (?,(?,(?,count))).
-        destruct fifo_full.
-        { now boolsimpl. }
-        { boolsimpl.
-          cbv [fifo_invariant] in H.
-          logical_simplify.
-          rewrite H4.
-          match goal with
-          | |- if ?B then _ else _ => destruct B
-          end.
-          { apply H1. }
-          trivial.
-          }
-      }
-      apply H.
-    }
-    { eapply step_realign_masked_invariant.
-      { now rewrite Hnew_realign_masked_contents. }
-      { now rewrite Hnew_realign_masked_contents. }
-      { now rewrite Hnew_realign_masked_contents. }
-      { cbv [realign_masked_fifo_pre] in Hpre. cbn in input, fifo_state.
-        destruct_products.
-        now cbn.
-      }
-      { apply H0. }
-    }
     all:
+      simplify_spec (realign_masked_fifo fifo_size);
+      simplify_spec realign;
+      assert ( (length new_fifo_contents =? fifo_size) = fifo_full);
+      [ destruct fifo_full; subst;
+        [ now rewrite Nat.eqb_refl
+        | apply Nat.eqb_neq; lia ]
+      |];
+      assert ( (length new_fifo_contents =? 0) = fifo_empty);
+      [ destruct fifo_empty;
+        [ rewrite H3; now rewrite Nat.eqb_refl
+        | apply Nat.eqb_neq; lia ]
+      |]; cbn [denote_type] in *.
+    all:
+      rewrite H6, H5 in *;
+      cbn [realign_spec];
+      use_correctness' realign;
+      cbn [denote_type] in *;
+      rewrite H7;
+      cbn [fst realign_spec];
+      cbv [realign_update_latched_valid realign_update_latched_bytes realign_update_state] in *;
+      autorewrite with tuple_if;
       cbn [fst snd];
-      erewrite (step_fifo (BitVec 32) fifo_size) with (new_contents := new_fifo_contents);
-      [ | trivial | now rewrite Hnew_fifo_contents |
-        cbn in input; destruct_products; cbn [fifo_pre fst snd];
-        destruct fifo_full; boolsimpl; try trivial;
-          boolsimpl;
-          cbv [fifo_invariant] in H;
-          logical_simplify;
-          rewrite H4;
-          match goal with
-          | |- if ?B then _ else _ => destruct B
-          end; try trivial
-      |  apply H ].
-    {
-      cbv [fifo_spec]; cbn [fst snd].
-      cbn [denote_type absorb_any] in *.
-      destr (length new_fifo_contents =? fifo_size).
-      { now rewrite E. }
-      { eapply step_fifo_invariant with (new_contents:=new_fifo_contents) in H.
-        { cbv [fifo_invariant] in H.
-          destruct (fst (step (fifo fifo_size) _ _)) as (?, (?, (?, ?))).
-          logical_simplify.
-          cbn [denote_type absorb_any] in *.
-          rewrite <- H4 in E.
-          rewrite <- H4.
-          lia.
-        }
-        { lia. }
-        { rewrite Hnew_fifo_contents. reflexivity. }
-        { cbn [fifo_pre fst snd].
-          destruct_products.
-          cbn in H.
-          destruct fifo_full.
-          { now boolsimpl. }
-          { boolsimpl.
-            cbv [fifo_invariant] in H.
-            logical_simplify.
-            rewrite H4.
-            match goal with
-            | |- if ?B then _ else _ => destruct B
-            end.
-            { apply H1. }
-            trivial.
-          }
-        }
-      }
-    }
-    {
-      cbv [fifo_spec]; cbn [fst snd].
-      cbn [denote_type absorb_any] in *.
-      destr (length new_fifo_contents =? 0).
-      { now rewrite E. }
-      { eapply step_fifo_invariant with (new_contents:=new_fifo_contents) in H.
-        { cbv [fifo_invariant] in H.
-          destruct (fst (step (fifo fifo_size) _ _)) as (?, (?, (?, ?))).
-          logical_simplify.
-          cbn [denote_type absorb_any] in *.
-          rewrite <- H4 in E.
-          rewrite <- H4.
-          lia.
-        }
-        { lia. }
-        { rewrite Hnew_fifo_contents. reflexivity. }
-        { cbn [fifo_pre fst snd].
-          destruct_products.
-          cbn in H.
-          destruct fifo_full.
-          { now boolsimpl. }
-          { boolsimpl.
-            cbv [fifo_invariant] in H.
-            logical_simplify.
-            rewrite H4.
-            match goal with
-            | |- if ?B then _ else _ => destruct B
-            end.
-            { apply H1. }
-            trivial.
-          }
-        }
-      }
-    }
+      use_correctness' (fifo (T:= BitVec 32) fifo_size);
+      destruct (length new_fifo_contents =? 0);[destruct H5|];
+        cbn [denote_type absorb_any] in *; rewrite H5; cbn [fst snd].
+
+    all: boolsimpl; push_length.
+    all: repeat rewrite Tauto.if_same.
+    all: destruct consumer_ready; destruct (length new_fifo_contents =? 0);
+        destruct (length new_fifo_contents =? fifo_size); boolsimpl;
+        destruct_one_match; try lia.
+    all: destruct_one_match; lia.
   Qed.
 
-  Lemma step_realign_masked_fifo
-      fifo_contents
-      realign_masked_contents
-      (input : denote_type (input_of (realign_masked_fifo fifo_size)))
-      (state : denote_type (state_of (realign_masked_fifo fifo_size))):
-
-    realign_masked_fifo_pre input state ->
-    realign_masked_fifo_invariant fifo_contents realign_masked_contents state ->
-    snd (step (realign_masked_fifo fifo_size) state input) = realign_masked_fifo_spec fifo_contents realign_masked_contents input.
+  Lemma realign_masked_fifo_output_correct : output_correct (realign_masked_fifo fifo_size).
   Proof.
-    intros.
-    destruct state as (top_state, (realign_masked_state, fifo_state)) eqn:?.
-    (* destruct realign_masked_state as (x0,(x1,(x2,(x3,x4)))). *)
-    destruct top_state as (is_last, (out_valid, (out_data, (out_length, (fifo_empty, fifo_full))))).
-    cbn in input, state.
-    cbv [realign_masked_fifo realign_masked_fifo_pre realign_masked_fifo_invariant K] in *.
-    intros. logical_simplify. cbn [fst snd] in *.
-    stepsimpl.
+    simplify_invariant (realign_masked_fifo fifo_size).
+    simplify_spec (realign_masked_fifo fifo_size).
+    cbn [absorb_any].
+
+    intros (data_valid, (data, (data_mask, (drain, (consumer_ready, []))))).
+    intros
+      ( (is_last, (out_valid, (out_data, (out_length, (fifo_empty, fifo_full)))))
+      , ( realign_state
+        , fifo_state)).
+    destruct realign_state as (?,(?,(?,(?,?)))) eqn:?.
+    destruct fifo_state as (?,(?,(?,?))) eqn:?.
+    intros (fifo_contents, ((realign_valid, realign_data), realign_contents)).
+
+    cbv [realign_masked_fifo K]; stepsimpl; push_length.
+
+    intros; logical_simplify.
+
+    cbv [update_repr realign_specification] in *; logical_simplify.
+
+    assert ( (length fifo_contents =? fifo_size) = fifo_full);
+    [ destruct fifo_full; subst;
+      [ now rewrite Nat.eqb_refl
+      | apply Nat.eqb_neq; lia ]
+    |].
+    assert ( (length fifo_contents =? 0) = fifo_empty);
+    [ destruct fifo_empty;
+      [ rewrite H3; now rewrite Nat.eqb_refl
+      | apply Nat.eqb_neq; lia ]
+    |]; cbn [denote_type] in *.
+
+    rewrite H6, H5 in *.
+
+    (* use_correctness. *)
+    match goal with
+    | |- context [ ?X ] =>
+      match X with
+      | match ?Y with pair _ _ => _ end =>
+        match Y with
+        | step ?c ?s ?i =>
+          find_correctness c;
+          rewrite (surjective_pairing Y);
+          use_correctness' c
+        end
+      end
+    end.
+    rewrite H7; clear H7.
+
     repeat (destruct_pair_let; cbn [fst snd]).
 
-    match goal with
-    | |- context [snd (step (fifo (T:=BitVec 32) fifo_size) ?X ?Y) ] =>
-      remember (snd (step (fifo (T:=BitVec 32) fifo_size) X Y)) as stepped_fifo
-    end.
-    match goal with
-    | |- context [ snd (step realign_masked ?X ?Y) ] =>
-      remember (snd (step realign_masked X Y)) as stepped_realign_maskeder
-    end.
+    cbn [fst realign_spec].
+    cbv [realign_update_latched_valid realign_update_latched_bytes realign_update_state] in *.
+    autorewrite with tuple_if.
+    cbn [fst snd].
+    use_correctness' (fifo (T:=BitVec 32) fifo_size).
+    simplify_invariant realign.
+    simplify_invariant (fifo (T:=BitVec 32) fifo_size).
+    cbv [realign_pre realign_invariant'] in *.
+    logical_simplify.
+    destruct (length fifo_contents =? 0);[destruct H5|]; rewrite H5; clear H5; cbn [fst snd].
+    1:
+      destr (
+       if drain
+       then
+        (1 <=? length fifo_contents)
+        || (if negb (negb (length fifo_contents =? fifo_size))
+            then realign_valid
+            else
+             (4 <=? length realign_contents)
+             || drain && true && consumer_ready && (1 <=? length realign_contents))
+       else 1 <=? length fifo_contents
+       ).
+    3:
+      destr (
+       if drain
+       then
+        (1 <=? length fifo_contents)
+        || (if negb (negb (length fifo_contents =? fifo_size))
+            then realign_valid
+            else
+             (4 <=? length realign_contents)
+             || drain && false && consumer_ready && (1 <=? length realign_contents))
+       else 1 <=? length fifo_contents
+       ).
 
-    assert (length fifo_contents =? fifo_size = fifo_full).
-    { destruct fifo_full.
-      { rewrite H2. apply Nat.eqb_refl. }
-      { apply Nat.eqb_neq. lia. }
+    { revert E; rewrite H3; destruct drain; destruct consumer_ready; boolsimpl;
+        destr (0=?fifo_size); try lia;
+        destr (1<=?0); try lia.
+      all: intro Hx; rewrite Hx; boolsimpl.
+      all: reflexivity.
     }
-    assert (length fifo_contents =? 0 = fifo_empty).
-    { destruct fifo_empty.
-      { rewrite H3. apply Nat.eqb_refl. }
-      { apply Nat.eqb_neq. lia. }
+    {
+      generalize dependent E.
+      rewrite H3; destruct drain; destruct consumer_ready; boolsimpl;
+        destr (0=?fifo_size); try lia;
+        destr (1<=?0); try lia.
+      1-2: intro Hx; eexists; rewrite Hx; reflexivity.
+      all: intros _; eexists; reflexivity.
     }
-
-    cbn [denote_type absorb_any] in *.
-    rewrite <- Heqstepped_realign_maskeder in *.
-    rewrite <- Heqstepped_fifo.
-
-    rewrite step_fifo with
-      (T:=BitVec 32) (fifo_size:=fifo_size)
-      (contents:=fifo_contents)
-      (new_contents:=realign_masked_fifo_update_fifo_contents fifo_contents input state)
-      in Heqstepped_fifo; cycle 1.
-    { trivial. }
-    { subst; reflexivity. }
-    { clear Heqstepped_fifo Heqstepped_realign_maskeder.
-      (* clear stepped_fifo stepped_realign_maskeder. *)
-      cbv [fifo_pre].
-      destruct_products.
-      destruct fifo_full; boolsimpl.
-      { trivial. }
-      {
-        match goal with
-        | |- if ?B then _ else _ => destruct B
-        end; try trivial.
-        cbn in H0.
-        logical_simplify.
-        now rewrite H6.
-      }
+    { revert E; destruct drain; destruct consumer_ready; boolsimpl;
+        destr (1 <=? length fifo_contents); try lia.
+      all: boolsimpl; reflexivity.
     }
-    { trivial. }
-    cbv [realign_masked_fifo_update_fifo_contents] in *.
-
-    rewrite step_realign_masked with
-      (latched_valid:=fst (fst realign_masked_contents))
-      (latched_bytes:=snd (fst realign_masked_contents))
-      (state_data:=snd realign_masked_contents)
-      in Heqstepped_realign_maskeder, Heqstepped_fifo; cycle 1.
-    { cbn [realign_masked_pre]; destruct_products; cbn; trivial. }
-    { subst; cbn [fst snd ]. trivial. }
-    { cbn [realign_masked_pre]; destruct_products; cbn; trivial. }
-    { subst; cbn [fst snd ]. trivial. }
-
-    cbv [realign_masked_fifo_spec].
-    destruct input as (data_valid, (data, (data_mask, (drain, (consumer_ready, u))))).
-    repeat (destruct_pair_let; cbn [fst snd]).
-    destruct u.
-    cbn [denote_type absorb_any] in *.
-    cbv [realign_masked_fifo_update_fifo_contents] in *.
-    cbn [fst snd] in *.
-    rewrite Heqd in Heqstepped_fifo; cbn [fst snd] in Heqstepped_fifo.
-    rewrite H4 in *.
-    rewrite H5 in *.
-    rewrite <- Heqstepped_realign_maskeder in *.
-    rewrite <- Heqstepped_fifo.
-    clear Heqstepped_realign_maskeder Heqstepped_fifo.
-    reflexivity.
+    {
+      generalize dependent E.
+      destruct drain; destruct consumer_ready; boolsimpl;
+        destr (1 <=? length fifo_contents); try lia.
+     }
   Qed.
+
+  Lemma realign_masked_fifo_at_reset : invariant_at_reset (realign_masked_fifo fifo_size).
+  Proof.
+    simplify_invariant (realign_masked_fifo fifo_size).
+    simplify_invariant (fifo (T:=BitVec 32) fifo_size).
+    simplify_invariant realign.
+    repeat destruct_pair_let; cbn [fst snd].
+    ssplit; cbn; try reflexivity.
+    1: push_length.
+    all: cbn; ssplit; lia.
+  Qed.
+
+  Existing Instances realign_masked_fifo_at_reset realign_masked_fifo_invariant_preserved
+           realign_masked_fifo_output_correct.
+
+  Global Instance realign_masked_fifo_correctness : correctness_for (realign_masked_fifo fifo_size).
+  Proof. constructor; typeclasses eauto. Defined.
+
 End RealignMaskedFifo.
